WIP A1 for merge_op

nondeterministic_dataflow/table_3/A1.thy
@@ -2,37 +2,189 @@ theory A1
 
 imports
   "../BNA_Operators"
+  "HOL-ex.Sketch_and_Explore"
 begin
 no_notation Sublist.parallel (infixl "\<parallel>" 50)
 
 section \<open>Axiom A1: Merge commutes with identity\<close>
 
+fun interleaves :: \<open>'a list \<Rightarrow> 'a list \<Rightarrow> 'a list \<Rightarrow> bool\<close> where
+  \<open>interleaves (x # xs) (y # ys) (z # zs) = (x = y \<and> interleaves xs ys (z # zs) \<or> x = z \<and> interleaves xs (y # ys) zs)\<close>
+| \<open>interleaves (x # xs) (y # ys) [] = (x # xs = y # ys)\<close>
+| \<open>interleaves (x # xs) [] (z # zs) = (x # xs = z # zs)\<close>
+| \<open>interleaves (_ # _) [] [] = False\<close>
+| \<open>interleaves [] [] [] = True\<close>
+| \<open>interleaves _ _ _ = False\<close>
+
+lemma interleaves_length:
+  \<open>interleaves xs ys zs \<Longrightarrow> length xs = length ys + length zs\<close>
+  by (induct xs ys zs rule: interleaves.induct) auto
+
+lemma interleaves_comm:
+  \<open>interleaves xs ys zs = interleaves xs zs ys\<close>
+  by (induction xs ys zs rule: interleaves.induct) auto
+
+abbreviation merged where \<open>merged xs ys zs \<equiv> interleaves (rev xs) (rev ys) (rev zs)\<close>
+
+lemma merged_length:
+  \<open>merged xs ys zs \<Longrightarrow> length xs = length ys + length zs\<close>
+  using interleaves_length by force
+
+lemma merged_empty:
+  \<open>merged [] ys zs \<Longrightarrow> ys = [] \<and> zs = []\<close>
+  using interleaves.elims(2) by blast
+
+lemma merged_comm:
+  \<open>merged xs ys zs = merged xs zs ys\<close>
+  using interleaves_comm by blast
+
+lemma merged_empty_left:
+  \<open>merged xs [] xs\<close>
+  using interleaves.elims(3) by fastforce
+
+lemma merged_empty_right:
+  \<open>merged xs xs []\<close>
+  using merged_comm merged_empty_left by blast
+
+lemma merge_append_L:
+  \<open>merged xs ys zs \<Longrightarrow> merged (xs @ [x]) (ys @ [x]) zs\<close>
+  using interleaves.elims(2) by fastforce
+
+lemma merge_append_R:
+  \<open>merged xs ys zs \<Longrightarrow> merged (xs @ [x]) ys (zs @ [x])\<close>
+  using interleaves.elims(2) by fastforce
+
+lemma progress_buffers1:
+  assumes \<open>p \<notin> defaults\<close>
+    and \<open>n = min (length (B1' p)) (length (B1 p))\<close>
+    and \<open>merged xs (take n (B1' p)) (take n (B1 p))\<close>
+  shows \<open>(step Tau)\<^sup>*\<^sup>* (map_op assoc id (map_op projl projr (comp_op Some (case_sum B2 B2')
+    (comp_op (\<lambda>_. None) (\<lambda>_. []) (id_op B1) (merge_op (case_sum B1' B1'')))
+    (merge_op (case_sum B3 B3')))))
+   (map_op assoc id (map_op projl projr (comp_op Some (case_sum (B2(p := [])) (B2'(p := [])))
+    (comp_op (\<lambda>_. None) (\<lambda>_. []) (id_op (B1(p := []))) (merge_op (case_sum (B1'(p := drop n (B1' p))) (B1''(p := drop n (B1'' p))))))
+    (merge_op (case_sum (B3(p := (B1 >> B2 >> B3) p)) (B3'(p := ((B2' >> B3') p) @ xs)))))))\<close>
+  sorry
+
 lemma A1_gen:
-  \<open>map_op projl projr (comp_op Some (case_sum buf2 buf2') (merge_op (case_sum buf1 buf1') \<parallel> id_op buf1'') (merge_op (case_sum buf3 buf3')))
-  ~ map_op (case_sum Inr Inl) id (map_op projl projr (comp_op Some (case_sum buf2' buf2) (id_op buf1'' \<parallel> merge_op (case_sum buf1 buf1')) (merge_op (case_sum buf3' buf3))))\<close>
-proof (coinduction arbitrary: buf1 buf1' buf1'' buf2 buf2' buf3 buf3' rule: bisim_coinduct_upto)
-  case BISIM
+  assumes \<open>A'' = A1'' >> A2'' >> A3''\<close>
+    and \<open>B = B1 >> B2 >> B3\<close>
+    and \<open>\<forall>p. \<exists>xs ys zs. merged xs (A'' p) ((A2 >> A3) p @ ys) \<and> merged ys (A1 p) (A1' p)
+      \<and> merged xs (B p) ((B2' >> B3') p @ zs) \<and> merged zs (B1' p) (B1'' p)\<close>
+  shows \<open>map_op projl projr (comp_op Some (case_sum A2 A2'')
+    (merge_op (case_sum A1 A1') \<parallel> id_op A1'')
+    (merge_op (case_sum A3 A3'')))
+  \<approx> map_op assoc id (map_op projl projr (comp_op Some (case_sum B2 B2')
+      (id_op B1 \<parallel> merge_op (case_sum B1' B1''))
+      (merge_op (case_sum B3 B3'))))\<close>
+  unfolding pcomp_op_def
+using assms proof (coinduction arbitrary: A'' A1 A1' A1'' A2 A2'' A3 A3'' B B1 B1' B1'' B2 B2' B3 B3' rule: wbisim_coinduct_upto'')
+  case SIM1
   then show ?case
-    unfolding sim_def pcomp_op_def
-  proof (intro allI conjI impI)
-    fix io :: "(('a + 'a) + 'a, 'a, 'b) IO"
-      and op1' :: "(('a + 'a) + 'a, 'a, 'b) op"
-    assume H: "step io (map_op projl projr (comp_op Some (case_sum buf2 buf2') (comp_op (\<lambda>_. None) (\<lambda>_. []) (merge_op (case_sum buf1 buf1')) (id_op buf1'')) (merge_op (case_sum buf3 buf3')))) op1'"
-    show "\<exists>op2'. step io (map_op (case_sum Inr Inl) id (map_op projl projr (comp_op Some (case_sum buf2' buf2) (comp_op (\<lambda>_. None) (\<lambda>_. []) (id_op buf1'') (merge_op (case_sum buf1 buf1'))) (merge_op (case_sum buf3' buf3))))) op2' \<and> bisim_cong (\<lambda>s t. \<exists>buf1 buf1' buf1'' buf2 buf2' buf3 buf3'. s = map_op projl projr (comp_op Some (case_sum buf2 buf2') (comp_op (\<lambda>_. None) (\<lambda>_. []) (merge_op (case_sum buf1 buf1')) (id_op buf1'')) (merge_op (case_sum buf3 buf3'))) \<and> t = map_op (case_sum Inr Inl) id (map_op projl projr (comp_op Some (case_sum buf2' buf2) (comp_op (\<lambda>_. None) (\<lambda>_. []) (id_op buf1'') (merge_op (case_sum buf1 buf1'))) (merge_op (case_sum buf3' buf3))))) op1' op2'"
-      using H by (auto elim!: step_map_op_elim step_comp_op_elim step_merge_op_elim step_id_op_cases) (fastforce intro: bc_base)+
-  next
-    fix io :: "(('a + 'a) + 'a, 'a, 'b) IO"
-      and op1' :: "(('a + 'a) + 'a, 'a, 'b) op"
-    assume H: "step io (map_op (case_sum Inr Inl) id (map_op projl projr (comp_op Some (case_sum buf2' buf2) (comp_op (\<lambda>_. None) (\<lambda>_. []) (id_op buf1'') (merge_op (case_sum buf1 buf1'))) (merge_op (case_sum buf3' buf3))))) op1'"
-    show "\<exists>op2'. step io (map_op projl projr (comp_op Some (case_sum buf2 buf2') (comp_op (\<lambda>_. None) (\<lambda>_. []) (merge_op (case_sum buf1 buf1')) (id_op buf1'')) (merge_op (case_sum buf3 buf3')))) op2' \<and> bisim_cong (\<lambda>s t. \<exists>buf1 buf1' buf1'' buf2 buf2' buf3 buf3'. s = map_op projl projr (comp_op Some (case_sum buf2 buf2') (comp_op (\<lambda>_. None) (\<lambda>_. []) (merge_op (case_sum buf1 buf1')) (id_op buf1'')) (merge_op (case_sum buf3 buf3'))) \<and> t = map_op (case_sum Inr Inl) id (map_op projl projr (comp_op Some (case_sum buf2' buf2) (comp_op (\<lambda>_. None) (\<lambda>_. []) (id_op buf1'') (merge_op (case_sum buf1 buf1'))) (merge_op (case_sum buf3' buf3))))) op1' op2'"
-      using H by (auto elim!: step_map_op_elim step_comp_op_elim step_merge_op_elim step_id_op_cases) (fastforce intro: bc_sym[OF bc_base])+
+    (* apply - explore (auto elim!: step_map_op_elim step_comp_op_elim step_merge_op_elim step_id_op_cases; hypsubst_thin?) *)
+  proof -
+    have "\<exists>op2'. wstep (Inp (Inl (Inl pb)) xb) (map_op assoc id (map_op projl projr (comp_op Some (case_sum B2 B2') (comp_op (\<lambda>_. None) (\<lambda>_. []) (id_op B1) (merge_op (case_sum B1' B1''))) (merge_op (case_sum B3 B3'))))) op2' \<and> wbisim_cong (\<lambda>op1 op2. \<exists>A'' A1 A1' A1'' A2 A2'' A3 A3''. op1 = map_op projl projr (comp_op Some (case_sum A2 A2'') (comp_op (\<lambda>_. None) (\<lambda>_. []) (merge_op (case_sum A1 A1')) (id_op A1'')) (merge_op (case_sum A3 A3''))) \<and> (\<exists>B1 B1' B1'' B2 B2' B3 B3'. op2 = map_op assoc id (map_op projl projr (comp_op Some (case_sum B2 B2') (comp_op (\<lambda>_. None) (\<lambda>_. []) (id_op B1) (merge_op (case_sum B1' B1''))) (merge_op (case_sum B3 B3')))) \<and> A'' = (A1'' >> A2'') >> A3'' \<and> (\<forall>p. \<exists>xs ys. merged xs (A'' p) (bulk_benq ys ((A2 >> A3) p)) \<and> merged ys (A1 p) (A1' p) \<and> (\<exists>zs. merged xs (((B1 >> B2) >> B3) p) (bulk_benq zs ((B2' >> B3') p)) \<and> merged zs (B1' p) (B1'' p))))) (map_op projl projr (comp_op Some (case_sum A2 A2'') (comp_op (\<lambda>_. None) (\<lambda>_. []) (merge_op (case_sum (BENQ pb xb A1) A1')) (id_op A1'')) (merge_op (case_sum A3 A3'')))) op2'"
+      if "\<forall>p. \<exists>xs ys. merged xs (((A1'' >> A2'') >> A3'') p) (bulk_benq ys ((A2 >> A3) p)) \<and> merged ys (A1 p) (A1' p) \<and> (\<exists>zs. merged xs (((B1 >> B2) >> B3) p) (bulk_benq zs ((B2' >> B3') p)) \<and> merged zs (B1' p) (B1'' p))"
+        and "pb \<notin> defaults"
+      for pb :: 'a
+        and xb :: 'b
+      using that
+      apply -
+      apply (drule spec[of _ pb])
+      apply (elim exE conjE)
+      subgoal for xs ys zs
+        apply (intro exI conjI)
+         apply fastforce
+        apply (rule wbc_base)
+        apply (intro exI conjI)
+           apply (rule refl)+
+        apply (intro allI)
+        subgoal for p
+          apply (cases \<open>p = pb\<close>)
+           apply (rule exI[of _ \<open>xs @ [xb]\<close>])
+           apply (rule exI[of _ \<open>ys @ [xb]\<close>])
+           apply (smt (verit, del_insts) BAPPEND_BENQ BENQ_access append_eq_appendI merge_append_L merge_append_R)
+          by (metis BAPPEND_BENQ BENQ_diff_access that(1))
+        done
+      done
+    moreover have "\<exists>op2'. wstep (Inp (Inl (Inr pb)) xb) (map_op assoc id (map_op projl projr (comp_op Some (case_sum B2 B2') (comp_op (\<lambda>_. None) (\<lambda>_. []) (id_op B1) (merge_op (case_sum B1' B1''))) (merge_op (case_sum B3 B3'))))) op2' \<and> wbisim_cong (\<lambda>op1 op2. \<exists>A'' A1 A1' A1'' A2 A2'' A3 A3''. op1 = map_op projl projr (comp_op Some (case_sum A2 A2'') (comp_op (\<lambda>_. None) (\<lambda>_. []) (merge_op (case_sum A1 A1')) (id_op A1'')) (merge_op (case_sum A3 A3''))) \<and> (\<exists>B1 B1' B1'' B2 B2' B3 B3'. op2 = map_op assoc id (map_op projl projr (comp_op Some (case_sum B2 B2') (comp_op (\<lambda>_. None) (\<lambda>_. []) (id_op B1) (merge_op (case_sum B1' B1''))) (merge_op (case_sum B3 B3')))) \<and> A'' = (A1'' >> A2'') >> A3'' \<and> (\<forall>p. \<exists>xs ys. merged xs (A'' p) (bulk_benq ys ((A2 >> A3) p)) \<and> merged ys (A1 p) (A1' p) \<and> (\<exists>zs. merged xs (((B1 >> B2) >> B3) p) (bulk_benq zs ((B2' >> B3') p)) \<and> merged zs (B1' p) (B1'' p))))) (map_op projl projr (comp_op Some (case_sum A2 A2'') (comp_op (\<lambda>_. None) (\<lambda>_. []) (merge_op (case_sum A1 (BENQ pb xb A1'))) (id_op A1'')) (merge_op (case_sum A3 A3'')))) op2'"
+      if "\<forall>p. \<exists>xs ys. merged xs (((A1'' >> A2'') >> A3'') p) (bulk_benq ys ((A2 >> A3) p)) \<and> merged ys (A1 p) (A1' p) \<and> (\<exists>zs. merged xs (((B1 >> B2) >> B3) p) (bulk_benq zs ((B2' >> B3') p)) \<and> merged zs (B1' p) (B1'' p))"
+        and "pb \<notin> defaults"
+      for pb :: 'a
+        and xb :: 'b
+      using that sorry
+    moreover have "\<exists>op2'. wstep (Inp (Inr pb) xb) (map_op assoc id (map_op projl projr (comp_op Some (case_sum B2 B2') (comp_op (\<lambda>_. None) (\<lambda>_. []) (id_op B1) (merge_op (case_sum B1' B1''))) (merge_op (case_sum B3 B3'))))) op2' \<and> wbisim_cong (\<lambda>op1 op2. \<exists>A'' A1 A1' A1'' A2 A2'' A3 A3''. op1 = map_op projl projr (comp_op Some (case_sum A2 A2'') (comp_op (\<lambda>_. None) (\<lambda>_. []) (merge_op (case_sum A1 A1')) (id_op A1'')) (merge_op (case_sum A3 A3''))) \<and> (\<exists>B1 B1' B1'' B2 B2' B3 B3'. op2 = map_op assoc id (map_op projl projr (comp_op Some (case_sum B2 B2') (comp_op (\<lambda>_. None) (\<lambda>_. []) (id_op B1) (merge_op (case_sum B1' B1''))) (merge_op (case_sum B3 B3')))) \<and> A'' = (A1'' >> A2'') >> A3'' \<and> (\<forall>p. \<exists>xs ys. merged xs (A'' p) (bulk_benq ys ((A2 >> A3) p)) \<and> merged ys (A1 p) (A1' p) \<and> (\<exists>zs. merged xs (((B1 >> B2) >> B3) p) (bulk_benq zs ((B2' >> B3') p)) \<and> merged zs (B1' p) (B1'' p))))) (map_op projl projr (comp_op Some (case_sum A2 A2'') (comp_op (\<lambda>_. None) (\<lambda>_. []) (merge_op (case_sum A1 A1')) (id_op (BENQ pb xb A1''))) (merge_op (case_sum A3 A3'')))) op2'"
+      if "\<forall>p. \<exists>xs ys. merged xs (((A1'' >> A2'') >> A3'') p) (bulk_benq ys ((A2 >> A3) p)) \<and> merged ys (A1 p) (A1' p) \<and> (\<exists>zs. merged xs (((B1 >> B2) >> B3) p) (bulk_benq zs ((B2' >> B3') p)) \<and> merged zs (B1' p) (B1'' p))"
+        and "pb \<notin> defaults"
+      for pb :: 'a
+        and xb :: 'b
+      using that sorry
+    moreover have "\<exists>op2'. wstep (Out pa (BHD pa A3)) (map_op assoc id (map_op projl projr (comp_op Some (case_sum B2 B2') (comp_op (\<lambda>_. None) (\<lambda>_. []) (id_op B1) (merge_op (case_sum B1' B1''))) (merge_op (case_sum B3 B3'))))) op2' \<and> wbisim_cong (\<lambda>op1 op2. \<exists>A'' A1 A1' A1'' A2 A2'' A3 A3''. op1 = map_op projl projr (comp_op Some (case_sum A2 A2'') (comp_op (\<lambda>_. None) (\<lambda>_. []) (merge_op (case_sum A1 A1')) (id_op A1'')) (merge_op (case_sum A3 A3''))) \<and> (\<exists>B1 B1' B1'' B2 B2' B3 B3'. op2 = map_op assoc id (map_op projl projr (comp_op Some (case_sum B2 B2') (comp_op (\<lambda>_. None) (\<lambda>_. []) (id_op B1) (merge_op (case_sum B1' B1''))) (merge_op (case_sum B3 B3')))) \<and> A'' = (A1'' >> A2'') >> A3'' \<and> (\<forall>p. \<exists>xs ys. merged xs (A'' p) (bulk_benq ys ((A2 >> A3) p)) \<and> merged ys (A1 p) (A1' p) \<and> (\<exists>zs. merged xs (((B1 >> B2) >> B3) p) (bulk_benq zs ((B2' >> B3') p)) \<and> merged zs (B1' p) (B1'' p))))) (map_op projl projr (comp_op Some (case_sum A2 A2'') (comp_op (\<lambda>_. None) (\<lambda>_. []) (merge_op (case_sum A1 A1')) (id_op A1'')) (merge_op (case_sum (BTL pa A3) A3'')))) op2'"
+      if "\<forall>p. \<exists>xs ys. merged xs (((A1'' >> A2'') >> A3'') p) (bulk_benq ys ((A2 >> A3) p)) \<and> merged ys (A1 p) (A1' p) \<and> (\<exists>zs. merged xs (((B1 >> B2) >> B3) p) (bulk_benq zs ((B2' >> B3') p)) \<and> merged zs (B1' p) (B1'' p))"
+        and "A3 pa \<noteq> []"
+        and "pa \<notin> defaults"
+      for pa :: 'a
+      using that
+      apply -
+      apply (drule spec[of _ pa])
+      apply (elim exE conjE)
+      subgoal for xs ys zs
+        apply (intro exI conjI)
+         apply (rule wstep_trans(1))
+          apply (rule progress_buffers1)
+            apply assumption
+        sorry
+      done
+    moreover have "\<exists>op2'. wstep (Out pa (BHD pa A3'')) (map_op assoc id (map_op projl projr (comp_op Some (case_sum B2 B2') (comp_op (\<lambda>_. None) (\<lambda>_. []) (id_op B1) (merge_op (case_sum B1' B1''))) (merge_op (case_sum B3 B3'))))) op2' \<and> wbisim_cong (\<lambda>op1 op2. \<exists>A'' A1 A1' A1'' A2 A2'' A3 A3''. op1 = map_op projl projr (comp_op Some (case_sum A2 A2'') (comp_op (\<lambda>_. None) (\<lambda>_. []) (merge_op (case_sum A1 A1')) (id_op A1'')) (merge_op (case_sum A3 A3''))) \<and> (\<exists>B1 B1' B1'' B2 B2' B3 B3'. op2 = map_op assoc id (map_op projl projr (comp_op Some (case_sum B2 B2') (comp_op (\<lambda>_. None) (\<lambda>_. []) (id_op B1) (merge_op (case_sum B1' B1''))) (merge_op (case_sum B3 B3')))) \<and> A'' = (A1'' >> A2'') >> A3'' \<and> (\<forall>p. \<exists>xs ys. merged xs (A'' p) (bulk_benq ys ((A2 >> A3) p)) \<and> merged ys (A1 p) (A1' p) \<and> (\<exists>zs. merged xs (((B1 >> B2) >> B3) p) (bulk_benq zs ((B2' >> B3') p)) \<and> merged zs (B1' p) (B1'' p))))) (map_op projl projr (comp_op Some (case_sum A2 A2'') (comp_op (\<lambda>_. None) (\<lambda>_. []) (merge_op (case_sum A1 A1')) (id_op A1'')) (merge_op (case_sum A3 (BTL pa A3''))))) op2'"
+      if "\<forall>p. \<exists>xs ys. merged xs (((A1'' >> A2'') >> A3'') p) (bulk_benq ys ((A2 >> A3) p)) \<and> merged ys (A1 p) (A1' p) \<and> (\<exists>zs. merged xs (((B1 >> B2) >> B3) p) (bulk_benq zs ((B2' >> B3') p)) \<and> merged zs (B1' p) (B1'' p))"
+        and "A3'' pa \<noteq> []"
+        and "pa \<notin> defaults"
+      for pa :: 'a
+      using that sorry
+    moreover have "\<exists>op2'. (step Tau)\<^sup>*\<^sup>* (map_op assoc id (map_op projl projr (comp_op Some (case_sum B2 B2') (comp_op (\<lambda>_. None) (\<lambda>_. []) (id_op B1) (merge_op (case_sum B1' B1''))) (merge_op (case_sum B3 B3'))))) op2' \<and> wbisim_cong (\<lambda>op1 op2. \<exists>A'' A1 A1' A1'' A2 A2'' A3 A3''. op1 = map_op projl projr (comp_op Some (case_sum A2 A2'') (comp_op (\<lambda>_. None) (\<lambda>_. []) (merge_op (case_sum A1 A1')) (id_op A1'')) (merge_op (case_sum A3 A3''))) \<and> (\<exists>B1 B1' B1'' B2 B2' B3 B3'. op2 = map_op assoc id (map_op projl projr (comp_op Some (case_sum B2 B2') (comp_op (\<lambda>_. None) (\<lambda>_. []) (id_op B1) (merge_op (case_sum B1' B1''))) (merge_op (case_sum B3 B3')))) \<and> A'' = (A1'' >> A2'') >> A3'' \<and> (\<forall>p. \<exists>xs ys. merged xs (A'' p) (bulk_benq ys ((A2 >> A3) p)) \<and> merged ys (A1 p) (A1' p) \<and> (\<exists>zs. merged xs (((B1 >> B2) >> B3) p) (bulk_benq zs ((B2' >> B3') p)) \<and> merged zs (B1' p) (B1'' p))))) (map_op projl projr (comp_op Some (case_sum A2 (BENQ pb (BHD pb A1'') A2'')) (comp_op (\<lambda>_. None) (\<lambda>_. []) (merge_op (case_sum A1 A1')) (id_op (BTL pb A1''))) (merge_op (case_sum A3 A3'')))) op2'"
+      if "\<forall>p. \<exists>xs ys. merged xs (((A1'' >> A2'') >> A3'') p) (bulk_benq ys ((A2 >> A3) p)) \<and> merged ys (A1 p) (A1' p) \<and> (\<exists>zs. merged xs (((B1 >> B2) >> B3) p) (bulk_benq zs ((B2' >> B3') p)) \<and> merged zs (B1' p) (B1'' p))"
+        and "pb \<notin> defaults"
+        and "A1'' pb \<noteq> []"
+      for pb :: 'a
+      using that sorry
+    moreover have "\<exists>op2'. (step Tau)\<^sup>*\<^sup>* (map_op assoc id (map_op projl projr (comp_op Some (case_sum B2 B2') (comp_op (\<lambda>_. None) (\<lambda>_. []) (id_op B1) (merge_op (case_sum B1' B1''))) (merge_op (case_sum B3 B3'))))) op2' \<and> wbisim_cong (\<lambda>op1 op2. \<exists>A'' A1 A1' A1'' A2 A2'' A3 A3''. op1 = map_op projl projr (comp_op Some (case_sum A2 A2'') (comp_op (\<lambda>_. None) (\<lambda>_. []) (merge_op (case_sum A1 A1')) (id_op A1'')) (merge_op (case_sum A3 A3''))) \<and> (\<exists>B1 B1' B1'' B2 B2' B3 B3'. op2 = map_op assoc id (map_op projl projr (comp_op Some (case_sum B2 B2') (comp_op (\<lambda>_. None) (\<lambda>_. []) (id_op B1) (merge_op (case_sum B1' B1''))) (merge_op (case_sum B3 B3')))) \<and> A'' = (A1'' >> A2'') >> A3'' \<and> (\<forall>p. \<exists>xs ys. merged xs (A'' p) (bulk_benq ys ((A2 >> A3) p)) \<and> merged ys (A1 p) (A1' p) \<and> (\<exists>zs. merged xs (((B1 >> B2) >> B3) p) (bulk_benq zs ((B2' >> B3') p)) \<and> merged zs (B1' p) (B1'' p))))) (map_op projl projr (comp_op Some (case_sum (BENQ pb (BHD pb A1) A2) A2'') (comp_op (\<lambda>_. None) (\<lambda>_. []) (merge_op (case_sum (BTL pb A1) A1')) (id_op A1'')) (merge_op (case_sum A3 A3'')))) op2'"
+      if "\<forall>p. \<exists>xs ys. merged xs (((A1'' >> A2'') >> A3'') p) (bulk_benq ys ((A2 >> A3) p)) \<and> merged ys (A1 p) (A1' p) \<and> (\<exists>zs. merged xs (((B1 >> B2) >> B3) p) (bulk_benq zs ((B2' >> B3') p)) \<and> merged zs (B1' p) (B1'' p))"
+        and "A1 pb \<noteq> []"
+        and "pb \<notin> defaults"
+      for pb :: 'a
+      using that sorry
+    moreover have "\<exists>op2'. (step Tau)\<^sup>*\<^sup>* (map_op assoc id (map_op projl projr (comp_op Some (case_sum B2 B2') (comp_op (\<lambda>_. None) (\<lambda>_. []) (id_op B1) (merge_op (case_sum B1' B1''))) (merge_op (case_sum B3 B3'))))) op2' \<and> wbisim_cong (\<lambda>op1 op2. \<exists>A'' A1 A1' A1'' A2 A2'' A3 A3''. op1 = map_op projl projr (comp_op Some (case_sum A2 A2'') (comp_op (\<lambda>_. None) (\<lambda>_. []) (merge_op (case_sum A1 A1')) (id_op A1'')) (merge_op (case_sum A3 A3''))) \<and> (\<exists>B1 B1' B1'' B2 B2' B3 B3'. op2 = map_op assoc id (map_op projl projr (comp_op Some (case_sum B2 B2') (comp_op (\<lambda>_. None) (\<lambda>_. []) (id_op B1) (merge_op (case_sum B1' B1''))) (merge_op (case_sum B3 B3')))) \<and> A'' = (A1'' >> A2'') >> A3'' \<and> (\<forall>p. \<exists>xs ys. merged xs (A'' p) (bulk_benq ys ((A2 >> A3) p)) \<and> merged ys (A1 p) (A1' p) \<and> (\<exists>zs. merged xs (((B1 >> B2) >> B3) p) (bulk_benq zs ((B2' >> B3') p)) \<and> merged zs (B1' p) (B1'' p))))) (map_op projl projr (comp_op Some (case_sum (BENQ pb (BHD pb A1') A2) A2'') (comp_op (\<lambda>_. None) (\<lambda>_. []) (merge_op (case_sum A1 (BTL pb A1'))) (id_op A1'')) (merge_op (case_sum A3 A3'')))) op2'"
+      if "\<forall>p. \<exists>xs ys. merged xs (((A1'' >> A2'') >> A3'') p) (bulk_benq ys ((A2 >> A3) p)) \<and> merged ys (A1 p) (A1' p) \<and> (\<exists>zs. merged xs (((B1 >> B2) >> B3) p) (bulk_benq zs ((B2' >> B3') p)) \<and> merged zs (B1' p) (B1'' p))"
+        and "A1' pb \<noteq> []"
+        and "pb \<notin> defaults"
+      for pb :: 'a
+      using that sorry
+    moreover have "\<exists>op2'. (step Tau)\<^sup>*\<^sup>* (map_op assoc id (map_op projl projr (comp_op Some (case_sum B2 B2') (comp_op (\<lambda>_. None) (\<lambda>_. []) (id_op B1) (merge_op (case_sum B1' B1''))) (merge_op (case_sum B3 B3'))))) op2' \<and> wbisim_cong (\<lambda>op1 op2. \<exists>A'' A1 A1' A1'' A2 A2'' A3 A3''. op1 = map_op projl projr (comp_op Some (case_sum A2 A2'') (comp_op (\<lambda>_. None) (\<lambda>_. []) (merge_op (case_sum A1 A1')) (id_op A1'')) (merge_op (case_sum A3 A3''))) \<and> (\<exists>B1 B1' B1'' B2 B2' B3 B3'. op2 = map_op assoc id (map_op projl projr (comp_op Some (case_sum B2 B2') (comp_op (\<lambda>_. None) (\<lambda>_. []) (id_op B1) (merge_op (case_sum B1' B1''))) (merge_op (case_sum B3 B3')))) \<and> A'' = (A1'' >> A2'') >> A3'' \<and> (\<forall>p. \<exists>xs ys. merged xs (A'' p) (bulk_benq ys ((A2 >> A3) p)) \<and> merged ys (A1 p) (A1' p) \<and> (\<exists>zs. merged xs (((B1 >> B2) >> B3) p) (bulk_benq zs ((B2' >> B3') p)) \<and> merged zs (B1' p) (B1'' p))))) (map_op projl projr (comp_op Some (case_sum (BTL pa A2) A2'') (comp_op (\<lambda>_. None) (\<lambda>_. []) (merge_op (case_sum A1 A1')) (id_op A1'')) (merge_op (case_sum (BENQ pa (BHD pa A2) A3) A3'')))) op2'"
+      if "\<forall>p. \<exists>xs ys. merged xs (((A1'' >> A2'') >> A3'') p) (bulk_benq ys ((A2 >> A3) p)) \<and> merged ys (A1 p) (A1' p) \<and> (\<exists>zs. merged xs (((B1 >> B2) >> B3) p) (bulk_benq zs ((B2' >> B3') p)) \<and> merged zs (B1' p) (B1'' p))"
+        and "A2 pa \<noteq> []"
+        and "pa \<notin> defaults"
+      for pa :: 'a
+      using that sorry
+    moreover have "\<exists>op2'. (step Tau)\<^sup>*\<^sup>* (map_op assoc id (map_op projl projr (comp_op Some (case_sum B2 B2') (comp_op (\<lambda>_. None) (\<lambda>_. []) (id_op B1) (merge_op (case_sum B1' B1''))) (merge_op (case_sum B3 B3'))))) op2' \<and> wbisim_cong (\<lambda>op1 op2. \<exists>A'' A1 A1' A1'' A2 A2'' A3 A3''. op1 = map_op projl projr (comp_op Some (case_sum A2 A2'') (comp_op (\<lambda>_. None) (\<lambda>_. []) (merge_op (case_sum A1 A1')) (id_op A1'')) (merge_op (case_sum A3 A3''))) \<and> (\<exists>B1 B1' B1'' B2 B2' B3 B3'. op2 = map_op assoc id (map_op projl projr (comp_op Some (case_sum B2 B2') (comp_op (\<lambda>_. None) (\<lambda>_. []) (id_op B1) (merge_op (case_sum B1' B1''))) (merge_op (case_sum B3 B3')))) \<and> A'' = (A1'' >> A2'') >> A3'' \<and> (\<forall>p. \<exists>xs ys. merged xs (A'' p) (bulk_benq ys ((A2 >> A3) p)) \<and> merged ys (A1 p) (A1' p) \<and> (\<exists>zs. merged xs (((B1 >> B2) >> B3) p) (bulk_benq zs ((B2' >> B3') p)) \<and> merged zs (B1' p) (B1'' p))))) (map_op projl projr (comp_op Some (case_sum A2 (BTL pa A2'')) (comp_op (\<lambda>_. None) (\<lambda>_. []) (merge_op (case_sum A1 A1')) (id_op A1'')) (merge_op (case_sum A3 (BENQ pa (BHD pa A2'') A3''))))) op2'"
+      if "\<forall>p. \<exists>xs ys. merged xs (((A1'' >> A2'') >> A3'') p) (bulk_benq ys ((A2 >> A3) p)) \<and> merged ys (A1 p) (A1' p) \<and> (\<exists>zs. merged xs (((B1 >> B2) >> B3) p) (bulk_benq zs ((B2' >> B3') p)) \<and> merged zs (B1' p) (B1'' p))"
+        and "A2'' pa \<noteq> []"
+        and "pa \<notin> defaults"
+      for pa :: 'a
+      using that sorry
+    ultimately show ?thesis
+      using SIM1 by (auto elim !: step_map_op_elim step_comp_op_elim step_merge_op_elim step_id_op_cases)
   qed
+next
+  case SIM2
+  then show ?case
+    (* apply - apply (auto elim !: step_map_op_elim step_comp_op_elim step_merge_op_elim step_id_op_cases; hypsubst_thin?) *)
+    sorry
 qed
 
 lemma A1:
-  \<open>(\<V> \<parallel> \<I>) \<bullet> \<V> ~ map_op (case_sum Inr Inl) id ((\<I> \<parallel> \<V>) \<bullet> \<V>)\<close>
+  \<open>(\<V> \<parallel> \<I>) \<bullet> \<V> \<approx> map_op assoc id ((\<I> \<parallel> \<V>) \<bullet> \<V>)\<close>
   unfolding scomp_op_def
   using A1_gen[of \<open>\<lambda>_. []\<close> \<open>\<lambda>_. []\<close> \<open>\<lambda>_. []\<close> \<open>\<lambda>_. []\<close> \<open>\<lambda>_. []\<close> \<open>\<lambda>_. []\<close> \<open>\<lambda>_. []\<close>]
-  by simp
+  sorry
 
 end
